syn/ex/Mesi/MesiL1L2LLExt.v
@@ -33,56 +33,60 @@ Definition dtr := fst (tree2Topo topo 0).
 (* 32KB L1: 2^8 * 2^2 * 32B *)
 Definition l1IndexSz: nat := 8.
 Definition l1LgWay: nat := 2.
-Definition l1LgULs: nat := 2.
-Definition l1LgDLs: nat := 1.
-Definition l1LgNumVictim: nat := l1LgULs.
-Definition l1Cache oidx := mesiCache oidx l1IndexSz l1LgWay l1LgNumVictim.
-Definition l1Mshrs oidx := mshrs oidx l1LgULs l1LgDLs.
+Definition l1NumPRqs: nat := 2.
+Definition l1NumCRqs: nat := 4.
+Definition l1PredNumVictim: nat := Nat.pred l1NumCRqs.
+Definition l1MshrSlotSz: nat := S (Nat.log2 (l1NumPRqs + l1NumCRqs - 1)).
+(** * FIXME: need to have a cache interface that does not use extended directories at all *)
+Definition l1Cache (oidx: IdxT): Modules :=
+  mesiCache oidx l1IndexSz l1LgWay 0 l1PredNumVictim l1MshrSlotSz.
+Definition l1Mshrs (oidx: IdxT): Modules := mshrs oidx l1NumPRqs l1NumCRqs.
 
 (* 128KB L2: 2^9 * 2^3 * 32B *)
 Definition l2IndexSz: nat := 9.
 Definition l2LgWay: nat := 3.
-Definition l2LgULs: nat := 2.
-Definition l2LgDLs: nat := 1.
-Definition l2LgNumVictim: nat := l2LgULs.
-Definition l2Cache oidx := mesiCache oidx l2IndexSz l2LgWay l2LgNumVictim.
-Definition l2Mshrs oidx := mshrs oidx l2LgULs l2LgDLs.
+Definition l2EDirLgWay: nat := 2.
+Definition l2NumPRqs: nat := 4.
+Definition l2NumCRqs: nat := 8.
+Definition l2PredNumVictim: nat := Nat.pred l2NumCRqs.
+Definition l2MshrSlotSz: nat := S (Nat.log2 (l2NumPRqs + l2NumCRqs - 1)).
+Definition l2Cache (oidx: IdxT): Modules :=
+  mesiCache oidx l2IndexSz l2LgWay l2EDirLgWay l2PredNumVictim l2MshrSlotSz.
+Definition l2Mshrs (oidx: IdxT): Modules := mshrs oidx l2NumPRqs l2NumCRqs.
 
 (* 512KB LL: 2^10 * 2^4 * 32B *)
 Definition llIndexSz: nat := 10.
 Definition llLgWay: nat := 4.
-Definition llLgULs: nat := 2.
-Definition llLgDLs: nat := 2.
-Definition llLgNumVictim: nat := llLgULs.
-Definition llCache oidx := mesiCache oidx llIndexSz llLgWay llLgNumVictim.
-Definition llMshrs oidx := mshrs oidx llLgULs llLgDLs.
+Definition llEDirLgWay: nat := 3.
+Definition llNumPRqs: nat := 16.
+Definition llNumCRqs: nat := 0.
+Definition llPredNumVictim: nat := Nat.pred llNumCRqs.
+Definition llMshrSlotSz: nat := S (Nat.log2 (llNumPRqs + llNumCRqs - 1)).
+Definition llCache (oidx: IdxT): Modules :=
+  mesiCache oidx llIndexSz llLgWay llEDirLgWay llPredNumVictim llMshrSlotSz.
+Definition llMshrs (oidx: IdxT): Modules := mshrs oidx llNumPRqs llNumCRqs.
 
 Definition kl1c (oidx: IdxT): Modules :=
-  ((compile_Object (H0 := MesiCompLineRW l1LgWay) dtr (existT _ _ (hl1 oidx)))
-     ++ l1Cache oidx ++ l1Mshrs oidx
-     ++ build_msg_outs_l1 oidx
-     ++ build_int_fifos oidx
-     ++ build_ext_fifos oidx)%kami.
+  ((build_controller_l1
+      (H2 := MesiCompLineRW l1LgWay 0) (mshrNumPRqs := l1NumPRqs) (mshrNumCRqs := l1NumCRqs)
+      l1IndexSz l1PredNumVictim (existT _ _ (hl1 oidx)))
+     ++ l1Cache oidx ++ l1Mshrs oidx)%kami.
 
+(** * FIXME: need to have [build_controller_li_2] *)
 Definition kl2c (oidx: IdxT): Modules :=
-  ((compile_Object (H0 := MesiCompLineRW l2LgWay) dtr (existT _ _ (hli topo oidx)))
-     ++ l2Cache oidx ++ l2Mshrs oidx
-     ++ build_msg_outs_li oidx
-     ++ build_int_fifos oidx)%kami.
+  ((build_controller_li_4
+      (H2 := MesiCompLineRW l2LgWay 0) (mshrNumPRqs := l2NumPRqs) (mshrNumCRqs := l2NumCRqs)
+      l2IndexSz l2PredNumVictim (existT _ _ (hli topo oidx)))
+     ++ l2Cache oidx ++ l2Mshrs oidx)%kami.
 
+(** * FIXME: need to have [build_controller_li_2] *)
 Definition kllc (oidx: IdxT): Modules :=
-  ((compile_Object (H0 := MesiCompLineRW llLgWay) dtr (existT _ _ (hli topo oidx)))
-     ++ llCache oidx ++ llMshrs oidx
-     ++ build_msg_outs_li oidx)%kami.
-(* ++ build_int_fifos oidx)%kami. *)
-
-Definition kmemc (oidx: IdxT): Modules :=
-  ((compile_Object (H0 := MesiCompLineRW 1) dtr (existT _ _ (hmem topo oidx)))
-     ++ mesiCache oidx 10 1 1 ++ mshrs oidx 1 1
-     ++ build_msg_outs_mem oidx)%kami.
+  ((build_controller_li_4
+      (H2 := MesiCompLineRW llLgWay 0) (mshrNumPRqs := llNumPRqs) (mshrNumCRqs := llNumCRqs)
+      llIndexSz llPredNumVictim (existT _ _ (hli topo oidx)))
+     ++ llCache oidx ++ llMshrs oidx)%kami.
 
 Definition k: Modules :=
-  (* ((kmemc 0) ++ *)
   ((kllc 0~>0)
      ++ ((kl2c 0~>0~>0) ++ (kl1c 0~>0~>0~>0 ++ kl1c 0~>0~>0~>1))
      ++ ((kl2c 0~>0~>1) ++ (kl1c 0~>0~>1~>0 ++ kl1c 0~>0~>1~>1)))%kami.
